\documentclass[11pt,a4paper]{article}
\usepackage[utf8]{inputenc}
\usepackage[english]{babel}
\usepackage{fontspec}
\usepackage{xunicode}
\usepackage{xltxtra}
\usepackage{polyglossia}
\usepackage{amsmath}
\usepackage{amsfonts}
\usepackage{amssymb}
\usepackage{graphicx}
\usepackage[left=2cm,right=2cm,top=2cm,bottom=2cm]{geometry}
\usepackage{afterpage}
\usepackage{xcolor}
\usepackage{pagecolor}
\usepackage{mathtools}
%\usepackage{fancyhdr}
\usepackage{hyperref}
\usepackage{blindtext}
\usepackage{mahjong}
\usepackage{amsthm}
\usepackage{chngcntr}
\usepackage{tikz}
\usepackage{bbold}
\usepackage{pdfpages}
\usepackage{xfrac}

\usepackage{stmaryrd}
\let\stmaryrdLightning\lightning

\author{Zehao Gao}

\begin{document}

\section*{Homework 2 solutions}

\paragraph{Question 1}

\begin{enumerate}

\item[]

\begin{align}
\left\{
\begin{array}{lcl}
x'=\frac{1}{\sqrt{1-\beta^2}}(x-\beta ct) \\
ct'=\frac{1}{\sqrt{1-\beta^2}}(ct-\beta t)
\end{array}
\right.
\end{align}

Taylor-expansion
\begin{align}
x'&=x-ct\beta \\
ct'&=x-t\beta
\end{align}

\end{enumerate}

\newpage

\paragraph{Question 2}

\begin{enumerate}

\item[]

Prove that every orthogonal transformation $A\in\mathbb{R}^2$ with $det(A)=1$ can be parameterized with $\vartheta$, so that
\begin{align}
A(\vartheta)=
\begin{bmatrix}
C_\vartheta & S_\vartheta \\
-S_\vartheta & C_\vartheta
\end{bmatrix}
\end{align}

\begin{proof}

We have
\begin{align}
A=
\begin{bmatrix}
a & b \\
c & d
\end{bmatrix}
\end{align}
with
\begin{align}
A^TA=\mathbb{1}
\end{align}
and 
\begin{align}
det(A)=1
\end{align}

so that
\begin{align}
\begin{bmatrix}
a & c \\
b & d
\end{bmatrix}
\begin{bmatrix}
a & b \\
c & d
\end{bmatrix}
=
\begin{bmatrix}
a^2+c^2 & ab+cd \\
ab+cd & b^2+d^2
\end{bmatrix}
=
\begin{bmatrix}
1 & 0 \\
0 & 1
\end{bmatrix}
\end{align}

therefore
\begin{align}
\left\{
\begin{array}{lcl}
a^2+c^2=b^2+d^2=1 \\
ad-cb=1 \\
ab+cd=0
\end{array}
\right.
\end{align}

substitute
\begin{align}
a=S_\vartheta\hspace{1em}
b=S_\varphi\hspace{1em}
c=C_\vartheta\hspace{1em}
d=C_\varphi
\end{align}

we get
\begin{align}
S^2_\vartheta+C^2_\vartheta=S^2_\varphi+C^2_\varphi&=1 \\
S_\vartheta C_\varphi-S_\varphi C_\vartheta=S_{\vartheta-\varphi}&=1 \\
S_\vartheta S_\varphi+C_\vartheta C_\varphi=C_{\vartheta-\varphi}&=0
\end{align}

therefore
\begin{align}
\vartheta-\varphi=\frac{\pi}{2}+2k\pi,\hspace{1em}k\in\mathbb{Z}
\end{align}
\begin{align}
S_\varphi=C_\vartheta,\hspace{1em}
C_\varphi=-S_\vartheta
\end{align}

\begin{align*}
A=
\begin{bmatrix}
S_\vartheta & C_\vartheta \\
C_\vartheta & -S_\vartheta
\end{bmatrix}
\end{align*}

\end{proof}

\end{enumerate}

\newpage

\paragraph{Question 3}

\begin{enumerate}

\item[]

\begin{align}
\vec{F}_g=-mg\hat{z}
\end{align}

\begin{align}
\vec{F}_R=-\alpha\vec{v}(t)
\end{align}

\begin{align}
(\vec{F}_g+\vec{F}_R)_z=(\vec{F})_z=m\ddot{z}=-mg-\alpha\dot{z}
\end{align}

\begin{align}
m\ddot{z}&=-mg-\alpha\dot{z} \\
m\frac{d^2}{dt^2}z&=-mg-\alpha\frac{d}{dt}z
\end{align}

Substitute $u=\dot{z}$
\begin{align}
m\frac{du}{dt}&=-mg-\alpha u \\
\frac{1}{g+\frac{\alpha}{m}u}du&=-dt \\
\int \frac{1}{g+\frac{\alpha}{m}u}du&=-\int dt \\
\frac{m}{\alpha}\ln(g+\frac{\alpha}{m}u)&=-t+C_0
\end{align}

with initial condition $\vec{v}(0)=\vec{v}_0$, we have $u(0)=\vec{v}_z$, therefore
\begin{align}
C_0=\frac{m}{\alpha}\ln(g+\frac{\alpha}{m}\vec{v}_z)
\end{align}

then we have
\begin{align}
\frac{m}{\alpha}\ln(g+\frac{\alpha}{m}u)&=-t+\frac{m}{\alpha}\ln(g+\frac{\alpha}{m}\vec{v}_z) \\
(g+\frac{\alpha}{m}u)^\frac{m}{\alpha}&=e^{-t}(g+\frac{\alpha}{m}\vec{v}_z)^\frac{m}{\alpha} \\
g+\frac{\alpha}{m}\frac{dz}{dt}&=e^{-\frac{\alpha}{m}t}(g+\frac{\alpha}{m}\vec{v}_z)
\end{align}

set $\frac{\alpha}{m}=k$
\begin{align}
gdt+kdz&=e^{-kt}(g+k\vec{v}_z)dt \\
\int kdz&=\int e^{-kt}(g+k\vec{v}_z)dt-\int gdt \\
kz&=-\frac{1}{k}e^{-kt}(g+k\vec{v}_z)-gt+C_1
\end{align}

\newpage

with initial condition $z(0)=0$
\begin{align}
C_1=\frac{1}{k}(g+k\vec{v}_z)
\end{align}

therefore
\begin{align}
z
&=\frac{1}{k^2}(g+k\vec{v}_z)-\frac{1}{k^2}e^{-kt}(g+k\vec{v}_z)-\frac{1}{k}gt \\
&=\frac{1}{k^2}[(g+k\vec{v}_z)(1-e^{-kt})-kgt]
\end{align}
with $k=\frac{\alpha}{m}$

\end{enumerate}

\end{document}
